{
 "cells": [
  {
   "attachments": {},
   "cell_type": "markdown",
   "metadata": {},
   "source": [
    "## All formulae for the scalar field on the schwarzchild space-time."
   ]
  },
  {
   "attachments": {},
   "cell_type": "markdown",
   "metadata": {},
   "source": [
    "## Spherically symmetric space times. \n",
    "\n",
    "We do de calculations using other names for the metric components and at the end substitute.\n",
    "\n",
    "$$ \n",
    "ds^2 = -adt^2 + 2b dtdr + c dr^2 + r^2 dΩ\n",
    "$$\n",
    "\n",
    "$$\n",
    "a = g(2-f),\\;\\;\\; b = g(f-1), \\;\\;\\; c = gf\n",
    "$$\n",
    "\n",
    "$$\n",
    "det(g_{\\mu\\nu}) = -(ac + b^2)r^4 \\sin ^2 \\theta= g^2r^4\n",
    "$$\n",
    "\n",
    "$$\n",
    "det_g := ac + b^2 = g^2\n",
    "$$\n",
    "\n",
    "$$\n",
    "g^{\\mu\\nu} = \\left(\n",
    "    \\begin{array}{cccc}\n",
    "    -c/g^2 & b/g^2 & 0 & 0 \\\\\n",
    "     b/g^2 & a/g^2 & 0 & 0 \\\\\n",
    "     0 & 0 & \\frac{1}{r^2} & 0 \\\\\n",
    "     0 & 0 & 0 & \\frac{1}{r^2 sin^2\\theta} \\\\\n",
    "    \\end{array}\n",
    "    \\right)\n",
    "$$\n",
    "\n",
    "\n",
    "\n"
   ]
  },
  {
   "attachments": {},
   "cell_type": "markdown",
   "metadata": {},
   "source": [
    "The equations for the scalar field are: \n",
    "\n",
    "\\begin{align}\n",
    "\\partial_t \\chi_+ &= \\partial_r \\chi_+ - \\frac{f-2}{fr}\\chi_- \\\\\n",
    "\\partial_t \\chi_- &= \\frac{f-2}{f}\\partial_r \\chi_- + \\frac{2}{f^2}\\chi_-(2(f-2)h - \\frac{f+g-2}{r} + \\frac{4}{fr}\\chi^2_+) - \\frac{\\chi_+}{r}\\\\\n",
    "\\end{align}\n",
    "\n",
    "Where\n",
    "\n",
    "$$ \n",
    "\\chi_{\\pm} = r\\frac{\\Pi \\pm \\Phi}{2}\n",
    "$$\n",
    "\n",
    "and \n",
    "\n",
    "\\begin{align}\n",
    "\\Pi &= f\\partial_t \\phi - (f-1)\\partial_r \\phi \\\\\n",
    "\\Phi &= \\partial_r \\phi \n",
    "\\end{align}\n",
    "\n",
    "Thus, \n",
    "\n",
    "$$\n",
    "\\partial_t \\phi = \\frac{1}{f}(\\Pi + (f-1)\\Phi) = \\frac{1}{rf}(f\\chi_+ - (f-2)\\chi_-)\n",
    "$$\n",
    "**la que sigue está mal, la saqué del arxiv, la anterior es del paper publicado y está bien** \n",
    "\n",
    "$$\n",
    "\\partial_t \\phi = \\Pi = \\frac{\\chi_+ + \\chi_-}{r}\n",
    "$$\n",
    "\n",
    "$$\n",
    "\\partial_r \\phi = \\frac{\\chi_+ - \\chi_-}{r}\n",
    "$$"
   ]
  },
  {
   "attachments": {},
   "cell_type": "markdown",
   "metadata": {},
   "source": [
    "## The wave equation is:\n",
    "\n",
    "$$\n",
    "-c ∂^2_t \\phi + 2b∂_t \\partial_r \\phi + a \\partial^2_r \\phi = -f ∂^2_t \\phi + 2(f-1)∂_t \\partial_r \\phi + (2-f) \\partial^2_r \\phi = 0\n",
    "$$\n",
    "\n",
    "Using $v:= ∂_t \\phi$, $w := ∂_r \\phi$ it becomes, \n",
    "\n",
    "$$\n",
    "-f \\sigma v + 2(f-1)\\sigma v + (2-f)w = 0\n",
    "$$\n",
    "\n",
    "Together with the equation, \n",
    "\n",
    "$$ \n",
    "\\sigma w = v\n",
    "$$\n",
    "We get the system:\n",
    "\n",
    "$$ \n",
    "\\left(\n",
    "    \\begin{array}{cc}\n",
    "    -f \\sigma + 2(f-1) & (2-f) \\\\\n",
    "     -1 & σ\n",
    "    \\end{array}\n",
    "\\right)\n",
    "$$\n",
    "\n",
    "The kernel is non-empty when the determinant vanishes,\n",
    "\n",
    "$$\n",
    "\\det = (-f \\sigma + 2(f-1))\\sigma + (2-f) = -f \\sigma^2 + 2(f-1)\\sigma + (2-f)  \n",
    "$$\n",
    "\n",
    "So\n",
    "\n",
    "$$ \n",
    "\\sigma_{\\pm} = \\frac{-2(f-1) \\mp \\sqrt{4(f-1)^2 + 4(2-f)f }}{-2f} = \\frac{(f-1) \\pm 1}{f}\n",
    "$$\n",
    "\n",
    "$$\n",
    "\\sigma_+ = 1 \\;\\;\\;\\;\\; \\sigma_- = \\frac{f-2}{f}\n",
    "$$\n",
    "\n",
    "$\\sigma_+ - \\sigma_- = 2/f$\n",
    "\n",
    "A base in the kernel is:\n",
    "\n",
    "$$\n",
    "U_{\\pm} = (\\sigma_{\\pm}, 1)\n",
    "$$\n",
    "\n",
    "The co-base is:\n",
    "\n",
    "$$\n",
    "Θ^{\\pm} = (1, -\\sigma_{\\mp})\\frac{1}{\\sigma_{\\pm} - \\sigma_{\\mp}}\n",
    "$$\n",
    "\n",
    "$$\n",
    "Θ^{\\pm}(U_{\\pm}) = (\\sigma_{\\pm} - \\sigma{\\mp})\\frac{1}{\\sigma_{\\pm} - \\sigma_{\\mp}} = 1 \\;\\;\\;\\;\\;\n",
    "Θ^{\\pm}(U_{\\mp}) = (\\sigma_{\\pm} - \\sigma{\\pm})\\frac{1}{\\sigma_{\\pm} - \\sigma_{\\mp}} = 0\n",
    "$$\n",
    "\n",
    "The modes are then: (form now on I changed the normalization so that they coincide with the ones in the paper)\n",
    "\n",
    "$$\n",
    "\\chi_+ = \\Theta^+(\\phi_t,\\phi_r) = (\\phi_t - \\frac{f-2}{f}\\phi_r)/2 \\;\\;\\;\\;\\;\\;\n",
    "\\chi_- = \\Theta^-(\\phi_t,\\phi_r) = (\\phi_t - \\phi_r)/2\n",
    "$$\n",
    "\n",
    "**I checked that they are indeed the two modes in the equations of the paper (to principal part only)but they do not coincide with any of the definitios we had!**\n",
    "\n",
    "$$\n",
    "\\phi_t = f\\chi_+ - (f-2)\\chi_- \\;\\;\\;\\;\\; \\phi_r = f(\\chi_+ - \\chi_-)\n",
    "$$"
   ]
  },
  {
   "attachments": {},
   "cell_type": "markdown",
   "metadata": {},
   "source": [
    "$\n",
    "\\begin{aligned}\n",
    "\\nabla_{\\sigma} \\phi \\nabla^{\\sigma} \\phi &= \\frac{1}{g^2}(-c \\phi_t^2 + 2b\\phi_t \\phi_r + a \\phi_r^2) \\\\\n",
    "&= \\frac{1}{g}(-f \\phi_t^2 + 2(f-1)\\phi_t \\phi_r + (2-f) \\phi_r^2) \\\\\n",
    "&= \\frac{1}{g}(-f[f\\chi_+ - (f-2)\\chi_-]^2  + 2(f-1)f[f\\chi_+ - (f-2)\\chi_-] [\\chi_+ - \\chi_-] + (2-f)f^2 [\\chi_+ - \\chi_-]^2) \\\\\n",
    "&= \\frac{1}{g}(2\\chi_+ \\chi_- [-2f] + \\chi_-^2 [-f(f-2)^2 + 2(f-1)f(f-2) - (f-2)f^2]) \\\\\n",
    "&= \\frac{-4f}{g} \\chi_+ \\chi_- \\\\\n",
    "\\end{aligned}\n",
    "$"
   ]
  },
  {
   "attachments": {},
   "cell_type": "markdown",
   "metadata": {},
   "source": [
    "$$\n",
    "T_{ab} = \\nabla_a \\phi \\nabla_b \\phi - \\frac{1}{2}g_{ab} \\nabla_c \\phi \\nabla^c \\phi\n",
    "$$"
   ]
  },
  {
   "attachments": {},
   "cell_type": "markdown",
   "metadata": {},
   "source": [
    "$\n",
    "\\begin{aligned}\n",
    "T_{tt} &= \\phi_t^2 + \\frac{1}{2}(2-f)[-4f\\chi_+ \\chi_-] \\\\\n",
    "        &= (f\\chi_+ - (f-2)\\chi_-)^2 + \\frac{1}{2}(2-f)[-4f\\chi_+ \\chi_- ]  \\\\\n",
    "        &= \\chi_+^2[f^2] + 2\\chi_+\\chi_-[-f(f-2) - (2-f)f] + \\chi_-^2[(f-2)^2] \\\\\n",
    "        &= f^2\\chi_+^2 + (f-2)^2\\chi_-^2 \\\\\n",
    "\\end{aligned}\n",
    "$\n",
    "\n",
    "$\n",
    "\\begin{aligned}\n",
    "T_{\\theta \\theta} &= \\frac{-r^2}{2g}[-4f\\chi_+ \\chi_- ]  \\\\\n",
    "&= -\\frac{r^2}{g}[-2f\\chi_+ \\chi_-]  \\\\\n",
    "\\end{aligned}\n",
    "$\n",
    "\n",
    "$\n",
    "\\begin{aligned}\n",
    "T_{rt} &= \\phi_t\\phi_r - \\frac{f-1}{2}[-4f\\chi_+ \\chi_-] \\\\\n",
    "        &= (f\\chi_+ - (f-2)\\chi_-)f(\\chi_+ - \\chi_-) + 2f(f-1) \\chi_+ \\chi_- \\\\\n",
    "        &= \\chi_+^2[f^2] + \\chi_+\\chi_-[-f^2-f(f-2) + 2f(f-1)] + \\chi_-^2[f(f-2)] \\\\\n",
    "        &= f^2 \\chi_+^2 + (f-2)f\\chi_-^2\n",
    "\\end{aligned}\n",
    "$\n",
    "\n",
    "$\n",
    "\\begin{aligned}\n",
    "T_{rr} &= \\phi_r\\phi_r - \\frac{f}{2}(-4f\\chi_+ \\chi_-) \\\\\n",
    "        &= f^2(\\chi_+ - \\chi_-)^2 + f[2f\\chi_+ \\chi_-  ] \\\\\n",
    "        &= f^2 \\chi_+^2 + 2\\chi_+\\chi_-[-f^2 +f^2] + \\chi_-^2[f^2] \\\\\n",
    "        &= f^2 \\chi_+^2 + f^2\\chi_-^2 \\\\\n",
    "\\end{aligned}\n",
    "$"
   ]
  },
  {
   "attachments": {},
   "cell_type": "markdown",
   "metadata": {},
   "source": [
    "$\n",
    "\\begin{aligned}\n",
    "& [T_{tr} - \\frac{f-1}{f}T_{rr}] \\\\\n",
    "&= f^2 \\chi_+^2 + (f-2)f\\chi_-^2 - \\frac{f-1}{f}( f^2 \\chi_+^2 + f^2\\chi_-^2)\\\\\n",
    "&= \\chi_+^2 [f^2(1 - \\frac{f-1}{f})]  + \\chi_-^2[f(f-2) - (f-1)f] \\\\\n",
    "&= f(\\chi_+^2  - \\chi_-^2)  \\\\\n",
    "\\end{aligned}\n",
    "$\n",
    "\n",
    "**This seems to agree (up to overall factors) with the calculation for the $C_g$ constraint.**\n",
    "\n",
    "\n",
    "$\n",
    "\\begin{aligned}\n",
    "& T_{tt}(f) - T_{rt}(f-1) = \\\\\n",
    "&= f[f^2\\chi_+^2 + (f-2)^2\\chi_-^2] - (f-1)[f^2 \\chi_+^2 + (f-2)f\\chi_-^2] \\\\\n",
    "&= \\chi_+^2[f^2(f - (f-1))]  + \\chi_-^2f(f-2)((f-2) - (f-1))\\\\\n",
    "&= f^2\\chi_+^2 -f(f-2)\\chi_-^2\n",
    "\\end{aligned}\n",
    "$\n",
    "\n",
    "$\n",
    "\\begin{aligned}\n",
    "&(2-f)[T_{tr} - \\frac{f-1}{f}T_{rr}] + [T_{tt}(f) - T_{rt}(f-1)] \\\\\n",
    "&= (2-f)f(\\chi_+^2  - \\chi_-^2) + (f^2\\chi_+^2  -(f-2)f\\chi_-^2) \\\\\n",
    "&= 2f\\chi_+^2 \n",
    "\\end{aligned}\n",
    "$\n",
    "\n",
    "**This result seems to agree up to an overall factor with the $C_f$ constraint equation.**"
   ]
  },
  {
   "attachments": {},
   "cell_type": "markdown",
   "metadata": {},
   "source": [
    "## Cuentas viejas y probablemente mal."
   ]
  },
  {
   "cell_type": "markdown",
   "metadata": {},
   "source": []
  }
 ],
 "metadata": {
  "kernelspec": {
   "display_name": "Julia 1.8.1",
   "language": "julia",
   "name": "julia-1.8"
  },
  "language_info": {
   "file_extension": ".jl",
   "mimetype": "application/julia",
   "name": "julia",
   "version": "1.8.1"
  },
  "orig_nbformat": 4
 },
 "nbformat": 4,
 "nbformat_minor": 2
}
